src/named/ElabWithPrefix.v
@@ -32,7 +32,7 @@ Section WithPrefix.
     that their sorts are wf.
      *)
     
-    Inductive elab_term : ctx -> exp -> exp -> sort -> Prop :=
+    Inductive elab_term : ctx -> term -> term -> sort -> Prop :=
     | elab_term_by : forall c n s es args c' t,
         In (n, term_rule c' args t) (l ++ l_pre) ->
         elab_args c s args es c' ->
@@ -44,7 +44,7 @@ Section WithPrefix.
     | elab_term_var : forall c n t,
         In (n, t) c ->
         elab_term c (var n) (var n) t
-    with elab_args : ctx -> list exp -> list string -> list exp -> ctx -> Prop :=
+    with elab_args : ctx -> list term -> list string -> list term -> ctx -> Prop :=
     | elab_args_nil : forall c, elab_args c [] [] [] []
     | elab_args_cons_ex : forall c s args es c' name e ee t,
         elab_term c e ee t[/with_names_from c' es/] ->
