src/named/Rule.v
@@ -6,105 +6,105 @@ Import ListNotations.
 Open Scope string.
 Open Scope list.
 From Utils Require Import Utils.
-From Named Require Import Exp.
+From Named Require Import Term.
 (*TODO: why does this generate warnings?*)
-Import Exp.Notations.
+Import Term.Notations.
 
 Inductive rule : Set :=
 | sort_rule :  ctx -> list string (*explicit args*) -> rule
 | term_rule :  ctx -> list string (*explicit args*) -> sort -> rule
 | sort_eq_rule : ctx -> sort -> sort -> rule
-| term_eq_rule : ctx -> exp -> exp -> sort -> rule.
-#[export] Hint Constructors rule : exp.
+| term_eq_rule : ctx -> term -> term -> sort -> rule.
+#[export] Hint Constructors rule : term.
 
 Definition lang := named_list rule.
 
 Lemma invert_eq_sort_rule_sort_rule c c' args args'
   : sort_rule c args = sort_rule c' args' <-> c = c' /\ args = args'.
 Proof. solve_invert_constr_eq_lemma. Qed.
-Hint Rewrite invert_eq_sort_rule_sort_rule : exp.
+Hint Rewrite invert_eq_sort_rule_sort_rule : term.
   
 Lemma invert_eq_sort_rule_term_rule c c' args args' t'
   : sort_rule c args = term_rule c' args' t' <-> False.
 Proof. solve_invert_constr_eq_lemma. Qed.
-Hint Rewrite invert_eq_sort_rule_term_rule : exp.
+Hint Rewrite invert_eq_sort_rule_term_rule : term.
 
 Lemma invert_eq_sort_rule_sort_eq_rule c c' args t1' t2'
   : sort_rule c args = sort_eq_rule c' t1' t2' <-> False.
 Proof. solve_invert_constr_eq_lemma. Qed.
-Hint Rewrite invert_eq_sort_rule_sort_eq_rule : exp.
+Hint Rewrite invert_eq_sort_rule_sort_eq_rule : term.
 
 Lemma invert_eq_sort_rule_term_eq_rule c c' args e1' e2' t
   : sort_rule c args = term_eq_rule c' e1' e2' t <-> False.
 Proof. solve_invert_constr_eq_lemma. Qed.
-Hint Rewrite invert_eq_sort_rule_term_eq_rule : exp.
+Hint Rewrite invert_eq_sort_rule_term_eq_rule : term.
   
 Lemma invert_eq_term_rule_sort_rule c c' args args' t
   : term_rule c args t = sort_rule c' args' <-> False.
 Proof. solve_invert_constr_eq_lemma. Qed.
-Hint Rewrite invert_eq_term_rule_sort_rule : exp.
+Hint Rewrite invert_eq_term_rule_sort_rule : term.
 
 Lemma invert_eq_term_rule_term_rule c c' args args' t t'
   : term_rule c args t = term_rule c' args' t' <-> c = c' /\ args = args' /\ t = t'.
 Proof. solve_invert_constr_eq_lemma. Qed.
-Hint Rewrite invert_eq_term_rule_term_rule : exp.
+Hint Rewrite invert_eq_term_rule_term_rule : term.
 
 Lemma invert_eq_term_rule_sort_eq_rule c c' args t t1' t2'
   : term_rule c args t = sort_eq_rule c' t1' t2' <-> False.
 Proof. solve_invert_constr_eq_lemma. Qed.
-Hint Rewrite invert_eq_term_rule_sort_eq_rule : exp.
+Hint Rewrite invert_eq_term_rule_sort_eq_rule : term.
 
 Lemma invert_eq_term_rule_term_eq_rule c c' args t e1' e2' t'
   : term_rule c args t = term_eq_rule c' e1' e2' t' <-> False.
 Proof. solve_invert_constr_eq_lemma. Qed.
-Hint Rewrite invert_eq_term_rule_term_eq_rule : exp.
+Hint Rewrite invert_eq_term_rule_term_eq_rule : term.
 
 
 Lemma invert_eq_sort_eq_rule_sort_rule c c' args' t1 t2
   : sort_eq_rule c t1 t2 = sort_rule c' args' <-> False.
 Proof. solve_invert_constr_eq_lemma. Qed.
-Hint Rewrite invert_eq_sort_eq_rule_sort_rule : exp.
+Hint Rewrite invert_eq_sort_eq_rule_sort_rule : term.
 
 Lemma invert_eq_sort_eq_rule_term_rule c c' args' t1 t2 t'
   : sort_eq_rule c t1 t2 = term_rule c' args' t' <-> False.
 Proof. solve_invert_constr_eq_lemma. Qed.
-Hint Rewrite invert_eq_sort_eq_rule_term_rule : exp.
+Hint Rewrite invert_eq_sort_eq_rule_term_rule : term.
 
 Lemma invert_eq_sort_eq_rule_sort_eq_rule c c' t1 t1' t2 t2'
   : sort_eq_rule c t1 t2 = sort_eq_rule c' t1' t2' <-> c = c' /\ t1 = t1' /\ t2 = t2'.
 Proof. solve_invert_constr_eq_lemma. Qed.
-Hint Rewrite invert_eq_sort_eq_rule_sort_eq_rule : exp.
+Hint Rewrite invert_eq_sort_eq_rule_sort_eq_rule : term.
 
 Lemma invert_eq_sort_eq_rule_term_eq_rule c c' t1 t2 e1' e2' t'
   : sort_eq_rule c t1 t2 = term_eq_rule c' e1' e2' t' <-> False.
 Proof. solve_invert_constr_eq_lemma. Qed.
-Hint Rewrite invert_eq_sort_eq_rule_term_eq_rule : exp.
+Hint Rewrite invert_eq_sort_eq_rule_term_eq_rule : term.
   
 Lemma invert_eq_term_eq_rule_sort_rule c c' e1 e2 args' t
   : term_eq_rule c e1 e2 t = sort_rule c' args' <-> False.
 Proof. solve_invert_constr_eq_lemma. Qed.
-Hint Rewrite invert_eq_term_eq_rule_sort_rule : exp.
+Hint Rewrite invert_eq_term_eq_rule_sort_rule : term.
 
 Lemma invert_eq_term_eq_rule_term_rule c c' args' t e1 e2 t'
   : term_eq_rule c e1 e2 t = term_rule c' args' t' <-> False.
 Proof. solve_invert_constr_eq_lemma. Qed.
-Hint Rewrite invert_eq_term_eq_rule_term_rule : exp.
+Hint Rewrite invert_eq_term_eq_rule_term_rule : term.
 
 Lemma invert_eq_term_eq_rule_sort_eq_rule c c' e1 e2 t t1' t2'
   : term_eq_rule c e1 e2 t = sort_eq_rule c' t1' t2' <-> False.
 Proof. solve_invert_constr_eq_lemma. Qed.
-Hint Rewrite invert_eq_term_eq_rule_sort_eq_rule : exp.
+Hint Rewrite invert_eq_term_eq_rule_sort_eq_rule : term.
 
 Lemma invert_eq_term_eq_rule_term_eq_rule c c' e1 e2 e1' e2' t t'
   : term_eq_rule c e1 e2 t = term_eq_rule c' e1' e2' t' <-> c = c' /\ e1 = e1' /\ e2 = e2' /\ t = t'.
 Proof. solve_invert_constr_eq_lemma. Qed.
-Hint Rewrite invert_eq_term_eq_rule_term_eq_rule : exp.
+Hint Rewrite invert_eq_term_eq_rule_term_eq_rule : term.
 
 
 (*Moved out of the module because Coq seems
   to include them at the the top level anyway
  *)
-Declare Custom Entry constr_conclusion.
+Declare Custom Entry constr_arg_list.
 
 Module Notations.
 
@@ -131,150 +131,103 @@ Check [TMP ------------------------------------------------].
 Definition with_rule_bar (rb : rule_bar) (r : string*rule) := r.
  *)
   
-  Declare Scope arule_scope.
-  Delimit Scope arule_scope with arule.
+  Declare Scope lang_scope.
+  Bind Scope lang_scope with lang.
 
-  (* TODO: is there a better way to do this that doesn't affect list parsing?
-     Current approach leads to 'only printing' notations
-   *)
-Notation "# s e .. e'" :=
-  (s, (cons e' .. (cons e nil) ..))%string
-  (in custom constr_conclusion at level 50,
-      s constr at level 0, e constr at level 0, e' constr at level 0,
-      format "# s  e  ..  e'"
-  ).
+  Declare Scope rule_scope.
+  Delimit Scope rule_scope with rule.
 
-Notation "# s" := (s, @nil string)%string
-  (in custom constr_conclusion at level 50,
-   s constr at level 0, format "# s").
+  Notation "{[l r1 ; .. ; r2 ]}" :=
+    ((cons r2 .. (cons r1 nil) ..))%rule
+      (format "'[' {[l '[hv' r1 ; '/' .. ; '/' r2 ']' ]} ']'") : lang_scope.
+  
+  Notation "e .. e'" :=
+    (cons e' .. (cons e nil) ..)%string
+    (in custom constr_arg_list at level 50,
+        e constr at level 0, e' constr at level 0,
+        format " '[hv' e  ..  e' ']'").
+
+  Notation "" :=
+    nil
+      (in custom constr_arg_list at level 0).
 
 
-Notation "'[s|' G ----------------------------------------------- cc 'srt' ]" :=
-  (fst cc, sort_rule G (snd cc))
-    (cc custom constr_conclusion at level 100,
+Notation "'[s|' G ----------------------------------------------- # s args 'srt' ]" :=
+  (s, sort_rule G args)
+    (s constr at level 0,
+     args custom constr_arg_list at level 100,
      G custom ctx at level 100,
-     format "'[' [s|  '[' G '//' ----------------------------------------------- '//' cc  'srt' ']' '//' ] ']'")
-  : arule_scope.
+     format "'[' [s|  '[' G '//' ----------------------------------------------- '//' '[' # s args  'srt' ']' ']' '//' ] ']'")
+  : rule_scope.
 
-
-Notation "'[s|' G ----------------------------------------------- # n 'srt' ]" :=
-  (n%string, sort_rule G [])
-    (n constr at level 0,
-     G custom ctx at level 100,
-     format "'[' [s|  '[' G '//' ----------------------------------------------- '//' # n  'srt' ']' '//' ] ']'",
-    only printing)
-  : arule_scope.
-
-Notation "'[s|' G ----------------------------------------------- # n a .. a' 'srt' ]" :=
-  (n%string, sort_rule G (cons a' .. (cons a nil) .. )%string)
-    (n constr at level 0,
-     G custom ctx at level 100,
-     a constr at level 0, a' constr at level 0,
-     format "'[' [s|  '[' G '//' ----------------------------------------------- '//' # n  a  ..  a'  'srt' ']' '//' ] ']'", only printing)
-  : arule_scope.
-
-Check [s| "x" : #"env", "y" : #"ty" %"x", "z" : #"ty" %"x"
+Check [s| "x" : #"env", "y" : #"ty" "x", "z" : #"ty" "x"
           -----------------------------------------------
-          #"foo" "y" "z" srt                    ]%arule.
-
-Eval compute in
-    [s| "x" : #"env", "y" : #"ty" %"x", "z" : #"ty" %"x"
-          -----------------------------------------------
-                      #"foo" "y" "z" srt                    ]%arule.
+          #"foo" "y" "z" srt                             ]%rule.
 
 Check [s| 
           -----------------------------------------------
-            #"env" srt                    ]%arule.
-
-
-Eval compute in
-    [s| 
-          -----------------------------------------------
-            #"env" srt                    ]%arule.
+            #"env" srt                                   ]%rule.
 
           
-Notation "[:| G ----------------------------------------------- cc : t ]" :=
-  (fst cc, term_rule G (snd cc) t)
-    (cc custom constr_conclusion at level 100,
+Notation "[:| G ----------------------------------------------- # s args : t ]" :=
+  (s, term_rule G args t)
+    (s constr at level 0,
+     args custom constr_arg_list at level 100,
      G custom ctx at level 100, t custom sort at level 100,
-     format "'[' [:|  '[' G '//' ----------------------------------------------- '//' '[' cc  '/' :  t ']' ']' '//' ] ']'") : arule_scope.
-
-Notation "'[:|' G ----------------------------------------------- # n : t ]" :=
-  (n%string, term_rule G [] t)
-    (n constr at level 0,
-     G custom ctx at level 100, t custom sort at level 100,
-     format "'[' [:|  '[' G '//' ----------------------------------------------- '//' # n  :  t ']' '//' ] ']'",
-    only printing)
-  : arule_scope.
-
-
-Notation "'[:|' G ----------------------------------------------- # n a .. a' : t ]" :=
-  (n%string, term_rule G (cons a' .. (cons a nil) .. )%string t)
-    (n constr at level 0,
-     a constr at level 0, a' constr at level 0,
-     G custom ctx at level 100, t custom sort at level 100,
-     format "'[' [:|  '[' G '//' ----------------------------------------------- '//' # n  a  ..  a'  :  t ']' '//' ] ']'", only printing)
-  : arule_scope.
+     format "'[' [:|  '[' G '//' ----------------------------------------------- '//' '[' # s args  '/' :  t ']' ']' '//' ] ']'") : rule_scope.
 
 Check [:| "G" : #"env",
-          "A" : #"ty" %"G",
-          "B" : #"ty" %"x",
-          "e" : #"el" (#"wkn" %"A" %"B")
+          "A" : #"ty" "G",
+          "B" : #"ty" "x",
+          "e" : #"el" (#"wkn" "A" "B")
           -----------------------------------------------
-          #"lam" "A" "e" : #"el" (#"->" %"A" %"B")]%arule.
+          #"lam" "A" "e" : #"el" (#"->" "A" "B")         ]%rule.
 
-Eval compute in
-     [:| "G" : #"env",
-          "A" : #"ty" %"G",
-          "B" : #"ty" %"x",
-          "e" : #"el" (#"wkn" %"A" %"B")
-          -----------------------------------------------
-          #"lam" "A" "e" : #"el" (#"->" %"A" %"B")]%arule.
 
 Check [:|
           -----------------------------------------------
-                      #"emp" : #"env"                   ]%arule.
+                      #"emp" : #"env"                     ]%rule.
 
 Eval compute in
      [:|
           -----------------------------------------------
-                      #"emp" : #"env"                   ]%arule.
+                      #"emp" : #"env"                    ]%rule.
 
 Check [:| "G" : #"env",
-           "A" : #"ty" %"G",
-           "B" : #"ty" %"x",
-           "e" : #"el" (#"wkn" %"A" %"B")
+           "A" : #"ty" "G",
+           "B" : #"ty" "x",
+           "e" : #"el" (#"wkn" "A" "B")
            -----------------------------------------------
-           #"lam" "e" : #"el" (#"->" %"A" %"B") ]%arule.
+           #"lam" "e" : #"el" (#"->" "A" "B")             ]%rule.
 
-Notation "'[s>' G ----------------------------------------------- ( s ) e1 = e2 ]" :=
+Notation "'[s=' G ----------------------------------------------- ( s ) e1 = e2 ]" :=
   (s%string, sort_eq_rule G e1 e2)
     (s constr at level 0, G custom ctx at level 100,
      e1 custom sort at level 100, e2 custom sort at level 100,
-     format "'[' [s>  '[' G '//' -----------------------------------------------  ( s ) '//' '[' e1 '/'  =  e2 ']' ']' '//' ] ']'")
-  : arule_scope.
+     format "'[' [s=  '[' G '//' -----------------------------------------------  ( s ) '//' '[' e1 '/'  =  e2 ']' ']' '//' ] ']'")
+  : rule_scope.
 
 
-Check [s> "G" : #"env", "A" : #"ty" %"G", "B" : #"ty" %"G",
-          "eq" : #"ty_eq" %"G" %"A" %"B" 
+Check [s= "G" : #"env", "A" : #"ty" "G", "B" : #"ty" "G",
+          "eq" : #"ty_eq" "G" "A" "B" 
           ----------------------------------------------- ("ty_eq_sort")
-          #"ty" %"G" %"A" = #"ty" %"G" %"B"
-      ]%arule.
+          #"ty" "G" "A" = #"ty" "G" "B"
+      ]%rule.
            
-Notation "[:> G ----------------------------------------------- ( s ) e1 = e2 : t ]" :=
+Notation "[:= G ----------------------------------------------- ( s ) e1 = e2 : t ]" :=
   (s%string, term_eq_rule G e1 e2 t)
     (s constr at level 0, G custom ctx at level 100,
      t custom sort at level 100,
-     e1 custom exp at level 100, e2 custom exp at level 100, 
-     format "'[' [:>  '[' G '//' -----------------------------------------------  ( s ) '//' '[' e1 '/'  =  e2 ']' '/'  :  t ']' '//' ] ']'")
-  : arule_scope.
+     e1 custom term at level 100, e2 custom term at level 100, 
+     format "'[' [:=  '[' G '//' -----------------------------------------------  ( s ) '//' '[' e1 '/'  =  e2 ']' '/'  :  t ']' '//' ] ']'")
+  : rule_scope.
 
 
-Check [:> "G" : #"env", "A" : #"ty" %"G", "B" : #"ty" %"G",
-          "eq" : #"ty_eq" %"G" %"A" %"B" 
+Check [:= "G" : #"env", "A" : #"ty" "G", "B" : #"ty" "G",
+          "eq" : #"ty_eq" "G" "A" "B" 
           ----------------------------------------------- ("ty_eq_sort")
-          %"A" = %"B" : #"ty" %"G"
-      ]%arule.
+          "A" = "B" : #"ty" "G"
+      ]%rule.
 
 End Notations.
 
@@ -283,16 +236,16 @@ End Notations.
 Definition ws_rule (r : rule) : bool :=
   match r with
   | {| c |- sort} => ws_ctx c
-  | {| c |- t} => ws_ctx c && ws_exp (size c) t
+  | {| c |- t} => ws_ctx c && ws_term (size c) t
   | {< c |- s1 <# s2} =>
     ws_ctx c
-           && ws_exp (size c) s1
-           && ws_exp (size c) s2
+           && ws_term (size c) s1
+           && ws_term (size c) s2
   | {< c |- e1 <# e2 .: s} =>
     ws_ctx c
-           && ws_exp (size c) e1
-           && ws_exp (size c) e2
-           && ws_exp (size c) s
+           && ws_term (size c) e1
+           && ws_term (size c) e2
+           && ws_term (size c) s
   end.
 
 Definition ws_lang : lang -> bool := List.forallb ws_rule.
@@ -321,7 +274,7 @@ Lemma rule_in_ws l n r : ws_lang l -> In (n,r) l -> ws_rule r.
 Proof using .
   induction l; 
     basic_goal_prep;
-    basic_exp_crush.
+    basic_term_crush.
 Qed.
 
 Lemma reconstruct_ws_lang l
@@ -329,11 +282,11 @@ Lemma reconstruct_ws_lang l
 Proof.
   eauto.
 Qed.
-#[export] Hint Resolve reconstruct_ws_lang : exp.
+#[export] Hint Resolve reconstruct_ws_lang : term.
 
 Lemma ws_lang_all_ws_rule l
   : ws_lang l -> all ws_rule (map snd l).
 Proof.
   unfold ws_lang; intuition.
 Qed.
-#[export] Hint Resolve ws_lang_all_ws_rule : exp.
+#[export] Hint Resolve ws_lang_all_ws_rule : term.
